\documentclass[10pt,a4paper]{article}
\usepackage[utf8]{inputenc}
\usepackage[english]{babel}
\usepackage{amsmath}
\usepackage{amsfonts}
\usepackage{amssymb}
\usepackage{amsthm}
\usepackage{enumitem}
\usepackage{listings}
\usepackage{pdfpages}
\usepackage{comment}
\usepackage{mathpartir}
\usepackage[top=2cm, bottom=3cm, left=1.5cm, right=1.5cm]{geometry}

\newcommand{\tu}{\textunderscore}

\lstset{
	tabsize=2,
	basicstyle=\small\ttfamily,
	columns=fixed,
	showstringspaces=false,
	breaklines=true,
	showtabs=false,
	showspaces=false,
	showstringspaces=false,
}

\newcounter{ExerciseCount}
\setcounter{ExerciseCount}{1}

\newcommand{\functionEx}[3]{
  Implement a function
  
  \vspace{0.15cm}
  \texttt{let #1 = #2}
   
   \vspace{0.15cm}
   #3
}
\newcommand{\reductionEx}[3]{
  \noindent
  Given the following untyped lambda-calculus expression:
  
  \begin{equation*}
  #1
  \end{equation*}
  
  \noindent
  replace the requested terms with the elements from the expression in the following lambda-calculus rule that evaluates it:
  
  \begin{mathpar}
  #2
  \end{mathpar}
  
  \begin{equation*}
  #3
  \end{equation*}
}

\newcommand{\varRule}{
  \begin{mathpar}
  \mprset{flushleft}
  \inferrule*[right=\quad (1)]{ }
  {x \rightarrow_{\beta} x}
  \end{mathpar}
}

\newcommand{\lambdaRule}{
  \begin{mathpar}
  \mprset{flushleft}
  \inferrule*[right=\quad (2)]{ }
  {(\lambda x \rightarrow t) \; u \rightarrow_{\beta} t[x \mapsto u]}
  \end{mathpar}
}

\newcommand{\appRule}{
  \begin{mathpar}
  \mprset{flushleft}
  \inferrule*[right=\quad (3)]{ t \rightarrow_{\beta} t' \wedge u \rightarrow u' \wedge t' \; u' \rightarrow_{\beta} v }
  {t \; u \rightarrow_{\beta} v}
  \end{mathpar}
}

\newcommand{\emptyPlace}{\tu\tu\tu}
\newcommand{\exercise}[1]{\noindent \textbf{Exercise \theExerciseCount:}
  
  \vspace{0.15cm}
 #1 \addtocounter{ExerciseCount}{1}
}

\title{Development 8 - Theory exercises}
\date {  }


\begin{document}
\maketitle
\large
\textbf{Beta-reduction rules:}
\normalsize

\vspace{0.5cm}
\textbf{Variables:}
\varRule

\vspace{0.5cm}
\textbf{Function application:}
\lambdaRule

\vspace{0.5cm}
\textbf{Application:}
\appRule

\vspace{0.5cm}

\exercise{
  \begin{align*}
  \begin{array}{l}
  x = x\\
  t = \lambda y \rightarrow x \; y\\
  u = \lambda y \rightarrow x \; y\\
  t[x \mapsto u] = \lambda y \rightarrow (\lambda y \rightarrow x \; y) \; y
  \end{array} 
  \end{align*}
}

\exercise{
  \begin{align*}
    \begin{array}{l}
    x = x\\
    t = \lambda x \rightarrow \lambda y \rightarrow y \; x\\
    u = A\\
    t[x \mapsto u] = \lambda x \rightarrow \lambda y \rightarrow y \; x \text{ \quad\quad mind the scope of x! }
    \end{array} 
    \end{align*}
}

\exercise{
  \begin{align*}
    \begin{array}{l}
    x = f\\
    t = \lambda g \rightarrow f\\
    u = \lambda x \rightarrow y \; x\\
    t[x \mapsto u] = \lambda g \rightarrow \lambda x \rightarrow y \; x
    \end{array} 
  \end{align*}
}

\exercise{
  \begin{align*}
    \begin{array}{l}
      x = x\\
      t = \lambda y \rightarrow ((\lambda z \rightarrow z) x)\\
      u = 0\\
      t[x \mapsto u] = \lambda y \rightarrow ((\lambda z \rightarrow z) \; 0)
      \end{array} 
    \end{align*}
}

\exercise{
   \begin{align*}
      \begin{array}{l}
        x = x\\
        t = \lambda x \; y \rightarrow y \; x\\
        u = 0\\
        t[x \mapsto u] = \lambda x \; y \rightarrow y \; x \text{\quad\quad mind the scope of x! }\\
        \end{array} 
    \end{align*}
}

\exercise{
  \begin{align*}
  \begin{array}{l}
     t = (\lambda x \; y \rightarrow y) \; 5 \\
     u = (\lambda x \rightarrow x) \; 3 \\
     t' = \lambda y \rightarrow y \\
     u'= 3 \\
     v = 
      \left \lbrace
      \begin{array}{l}
      (\lambda y \rightarrow y) \; 3 \rightarrow_\beta \quad\\
      3 
      \end{array} \right.
   \end{array}
  \end{align*}
}

\exercise{
  \begin{align*}
    \begin{array}{l}
       t = (\lambda f \; g \rightarrow f) (\lambda x \rightarrow x)\\
       u = 5 \\
       t' = \lambda g \rightarrow \lambda x \rightarrow x \\
       u'= 5 \\
       v = \left \lbrace \begin{array}{l}
          (\lambda g \rightarrow \lambda x \rightarrow x) \; 5 \rightarrow_{\beta}\\
          \lambda x \rightarrow x
          \end{array} \right.
     \end{array}
    \end{align*}
}

\exercise{
  \begin{align*}
      \begin{array}{l}
         t = ((\lambda f \; g \rightarrow g) \; ((\lambda x \; y \rightarrow \; y) \; 3))\\
         u = (\lambda f \; g \rightarrow f) \\
         t' = \left\lbrace
          \begin{array}{l}
          (\lambda f \; g \rightarrow g) \; ((\lambda x \; y \rightarrow \; y) \; 3) \rightarrow_\beta\\
          (\lambda f \; g \rightarrow g) \; (\lambda y \rightarrow \; y) \rightarrow_\beta\\
          \lambda g \rightarrow g
          \end{array} \right. \\
         u'= (\lambda f \; g \rightarrow f) \\
         v = \left \lbrace \begin{array}{l}
            (\lambda g \rightarrow g) \; (\lambda f \; g \rightarrow f) \rightarrow_{\beta} \\
            (\lambda f \; g \rightarrow f)
            \end{array} \right.
       \end{array}
      \end{align*}
}

\exercise{
  \begin{align*}
        \begin{array}{l}
           t = ((\lambda x \; y \; z \rightarrow y \; z \; x) \; (\lambda x \rightarrow x)) (\lambda y \; x \rightarrow x \; y)\\
           u = 3 \\
           t' = \left\lbrace
            \begin{array}{l}
            ((\lambda x \; y \; z \rightarrow y \; z \; x) \; (\lambda x \rightarrow x)) (\lambda y \; x \rightarrow x \; y) \rightarrow_\beta\\
            (\lambda y \; z \rightarrow y \; z \; (\lambda x \rightarrow x)) (\lambda y \; x \rightarrow x \; y) \rightarrow_\beta\\
            \lambda z \rightarrow ((\lambda y \; x \rightarrow x \; y) \; z) \; (\lambda x \rightarrow x) \rightarrow_{\beta}\\
            \lambda z \rightarrow (\lambda x \rightarrow x \; z) \; (\lambda x \rightarrow x)\\
            \lambda z \rightarrow (\lambda x \rightarrow x) \; z \\
            \lambda z \rightarrow z
            \end{array} \right. \\
           u'= 3 \\
           v = \left \lbrace \begin{array}{l}
              (\lambda z \rightarrow z) \; 3 \rightarrow_{\beta}\\
              3
              \end{array} \right.
         \end{array}
        \end{align*}
}
\newpage
\exercise{
  \begin{align*}
    \begin{array}{l}
       t = \lambda x \; y \rightarrow x\\
       u = ((\lambda f \; g \rightarrow g) \; (\lambda x \rightarrow x)) \; 3 \\
       t' = \lambda x \; y \rightarrow x \\
       u'= \left\lbrace \begin{array}{l}
           ((\lambda f \; g \rightarrow g) \; (\lambda x \rightarrow x)) \; 3 \rightarrow_{\beta}\\
           (\lambda g \rightarrow g) \; 3 \\
           3
           \end{array} \right. \\
       v = \left \lbrace \begin{array}{l}
           (\lambda x \; y \rightarrow x) \; 3 \rightarrow_{\beta}\\
           \lambda y \rightarrow 3
          \end{array} \right.
     \end{array}
    \end{align*}
}

\end{document}